trunk/color/Term/SimpleType/TermsEta.v
@@ -9,7 +9,7 @@ The eta-reduction relation of simply typed lambda-calculus.
 
 Set Implicit Arguments.
 
-Require Import Relations RelExtras ListExtras Omega.
+Require Import Relations RelExtras ListExtras.
 Require TermsBeta.
 
 Module TermsEta (Sig : TermsSig.Signature).
